Progress on Mail conversion; having trouble with DeliverImpl proofs.
I can't get the Ltac to do quite as much as it used to, so there are
some additional subgoals in createwritetmp_right_mover that I don't
understand. Similar subgoals are also showing up towards the end of
unlinktmp_left_mover.

I got the conversion for MailServerComposedImpl to go through, but am
having type issues with some of the definitions in
MailServerLockAbsImpl.

src/Mail/MailServerComposedImpl.v
@@ -2,46 +2,45 @@ Require Import CSPEC.
 Require Import MailServerAPI.
 Require Import MailServerComposedAPI.
 
-Module MailServerComposedImpl' <:
-  LayerImplMoversT
-    MailServerComposedState
-    MailServerHOp        MailServerHAPI
-    MailServerComposedOp MailServerComposedAPI.
+Module MailServerComposedImpl'.
 
   Import MailServerComposedOp.
 
   (* START CODE *)
 
-  Definition compile_op T (op : MailServerComposedOp.Op T) : proc MailServerHOp.Op T :=
+  Definition compile_op T (op : MailServerComposedOp.Op T) : proc MailServerHOp T :=
     match op with
     | Deliver u m => Call (Slice u (MailServerOp.Deliver m))
     | Pickup u => Call (Slice u (MailServerOp.Pickup))
-    | CheckUser u => Call (CheckSlice u)
+    | CheckUser u => Call (CheckSlice (u: UserIdx.idx))
     | Delete u id => Call (Slice u (MailServerOp.Delete id))
-    | Ext extop => Call (Slice nouser (MailServerOp.Ext extop))
+    | Ext extop => Call (Slice (nouser: validIndexT UserIdx.idx) (MailServerOp.Ext extop))
     end.
 
   (* END CODE *)
 
   Theorem compile_op_no_atomics :
-    forall `(op : _ T),
+    forall T (op : _ T),
       no_atomics (compile_op op).
   Proof.
     destruct op; simpl; eauto.
   Qed.
 
   Ltac step_inv :=
+    cbn [Layer.step MailServerHAPI] in *;
+    cbn [Layer.step MailServerComposedAPI.l] in *;
     match goal with
-    | H : MailServerHAPI.step _ _ _ _ _ _ |- _ =>
+    | H : MailServerHAPI.(Layer.step) _ _ _ _ _ _ |- _ =>
       inversion H; clear H; subst; repeat sigT_eq
-    | H : MailServerAPI.step _ _ _ _ _ _ |- _ =>
+    | H : MailServerAPI.l.(Layer.step) _ _ _ _ _ _ |- _ =>
       inversion H; clear H; subst; repeat sigT_eq
     end; intuition idtac.
 
   Hint Constructors MailServerComposedAPI.xstep.
 
+  Print MailServerHAPI.
   Theorem compile_correct :
-    compile_correct compile_op MailServerHAPI.step MailServerComposedAPI.step.
+    compile_correct compile_op MailServerHAPI.(Layer.step) MailServerComposedAPI.l.(Layer.step).
   Proof.
     unfold compile_correct; intros.
     destruct op.
@@ -49,8 +48,7 @@ Module MailServerComposedImpl' <:
     all: repeat step_inv.
     all: unfold MailServerComposedAPI.step.
     all: unfold user in *.
-    all: unfold UserIdx.indexT in *.
-    all: repeat sigT_eq.
+    all: unfold UserIdx.idx in *.
     all: try destruct_validIndex.
     all: try rewrite hadd_hget_eq.
     all: eauto.
@@ -61,20 +59,24 @@ Module MailServerComposedImpl' <:
   Qed.
 
   Theorem ysa_movers : forall `(op : _ T),
-    ysa_movers MailServerHAPI.step (compile_op op).
+    ysa_movers MailServerHAPI.(Layer.step) (compile_op op).
   Proof.
     destruct op; simpl; eauto.
   Qed.
 
-  Definition initP_compat : forall s, MailServerHAPI.initP s ->
-                                 MailServerComposedAPI.initP s :=
+  Definition initP_compat : forall s, MailServerHAPI.(Layer.initP) s ->
+                                 MailServerComposedAPI.l.(Layer.initP) s :=
     ltac:(auto).
 
+  Definition l : LayerImplMoversT.t MailServerHAPI MailServerComposedAPI.l.
+    refine {| LayerImplMoversT.ysa_movers := @ysa_movers;
+              LayerImplMoversT.initP_compat := initP_compat;
+              LayerImplMoversT.compile_correct := compile_correct;
+              LayerImplMoversT.compile_op := compile_op;
+              LayerImplMoversT.compile_op_no_atomics := compile_op_no_atomics; |}.
+    Defined.
+    
 End MailServerComposedImpl'.
 
-Module MailServerComposedImpl :=
-  LayerImplMovers
-    MailServerComposedState
-    MailServerHOp        MailServerHAPI
-    MailServerComposedOp MailServerComposedAPI
-    MailServerComposedImpl'.
+Definition MailServerComposedImpl :=
+ LayerImplMovers.t MailServerComposedImpl'.l.
