src/Mail/MailServerLockAbsImpl.v
@@ -2,20 +2,18 @@ Require Import CSPEC.
 Require Import MailServerAPI.
 Require Import MailServerLockAbsAPI.
 
-Module MailServerLockAbsImpl' <:
-  HLayerImplAbsT MailServerOp
-    MailServerLockAbsState MailServerLockAbsAPI
-    MailServerState MailServerAPI.
+Module MailServerLockAbsImpl'.
 
   Import MailServerLockAbsState.
+  Import Layer.
 
   Definition absR (s1 : MailServerLockAbsState.State) (s2 : MailServerState.State) :=
     MailServerLockAbsState.maildir s1 = s2.
 
-  Hint Extern 1 (MailServerAPI.step _ _ _ _ _ _) => econstructor.
+  Hint Extern 1 (MailServerAPI.l.(step) _ _ _ _ _ _) => econstructor.
 
   Theorem absR_ok :
-    op_abs absR MailServerLockAbsAPI.step MailServerAPI.step.
+    op_abs absR MailServerLockAbsAPI.l.(step) MailServerAPI.l.(step).
   Proof.
     unfold op_abs; intros.
     unfold absR in *.
@@ -23,10 +21,19 @@ Module MailServerLockAbsImpl' <:
     all: eauto.
   Qed.
 
-  Definition initP_map (s1: MailServerLockAbsState.State) : {s2:MailServerState.State | initP s1 -> absR s1 s2 /\ MailServerState.initP s2}.
+  Set Printing All.
+  Print MailServerLockAbsState.
+
+  Definition initP_map (s1: MailServerLockAbsState.State) :
+    {s2: MailServerState.State | initP s1 -> absR s1 s2 /\ MailServerState.initP s2}.
     exists (maildir s1).
     unfold initP, absR, MailServerState.initP; eauto.
   Defined.
+
+Definitnion t : 
+  HLayerImplAbsT MailServerOp
+    MailServerLockAbsState MailServerLockAbsAPI
+    MailServerState MailServerAPI.
 
 End MailServerLockAbsImpl'.
 
